explored issues with halting a little bit

theories/Secure/SecureEq.v
@@ -23,6 +23,7 @@ From ITree Require Import
      Events.State
      Events.StateFacts
      Core.Divergence
+     Dijkstra.TracesIT
 .
 
 From Paco Require Import paco.
@@ -31,6 +32,8 @@ Import Monads.
 Import MonadNotation.
 Local Open Scope monad_scope.
 
+
+Variant nonempty (A : Type) : Prop := ne (a : A).
 
 Class Preorder :=
   {
@@ -41,9 +44,10 @@ Class Preorder :=
 (* will need more propositional constrainst on Preorders *)
 
 Section SecureUntimed.
-  Context {E : Type -> Type} {R1 R2 : Type} (RR : R1 -> R2 -> Prop).
-  Context {Label : Preorder}.
+  Context {E : Type -> Type} {R1 R2 : Type}.
+  Context (Label : Preorder).
   Context (priv : forall A, E A -> L).
+  Context (RR : R1 -> R2 -> Prop).
 
   Inductive secure_eqitF (b1 b2 : bool) (l : L) vclo (sim : itree E R1 -> itree E R2 -> Prop) : itree' E R1 -> itree' E R2 -> Prop := 
 
@@ -55,10 +59,12 @@ Section SecureUntimed.
     (* info_flow protecting coinductive constructors *)
     | EqVisPriv {A} (e : E A) k1 k2 (SECCHECK : leq (priv A e) l) : 
         ((forall a, vclo sim (k1 a) (k2 a) : Prop)) -> secure_eqitF b1 b2 l vclo sim (VisF e k1) (VisF e k2)
-    | EqVisUnPrivLCo {A} (e : E A) k1 t2 (SECCHECK : ~ leq (priv A e) l) :
+    | EqVisUnPrivTauLCo {A} (e : E A) k1 t2 (SECCHECK : ~ leq (priv A e) l) :
         (forall a, vclo sim (k1 a) t2) -> secure_eqitF b1 b2 l vclo sim (VisF e k1) (TauF t2)
-    | EqVisUnPrivRCo {A} (e : E A) t1 k2 (SECCHECK : ~ leq (priv A e) l) :
+    | EqVisUnPrivTauRCo {A} (e : E A) t1 k2 (SECCHECK : ~ leq (priv A e) l) :
         (forall a, vclo sim t1 (k2 a)) -> secure_eqitF b1 b2 l vclo sim (TauF t1) (VisF e k2)
+    | EqVisUnPrivVisCo {A B} (e1 : E A) (e2 : E B) k1 k2 (SECCHECK1 : ~ leq (priv A e1) l) (SECCHECK2 : ~ leq (priv B e2) l) :
+        (forall a b, vclo sim (k1 a) (k2 b)) -> secure_eqitF b1 b2 l vclo sim (VisF e1 k1) (VisF e2 k2)
     (* info_flow protecting inductive constructors *)
     | EqVisUnPrivLInd {A} (e : E A) k1 t2 (CHECK : b1) (SECCHECK : ~ leq (priv A e) l) :
         (forall a, secure_eqitF b1 b2 l vclo sim (observe (k1 a)) (observe t2) ) ->
@@ -66,6 +72,9 @@ Section SecureUntimed.
     | EqVisUnPrivRLInd {A} (e : E A) t1 k2 (CHECK : b2) (SECCHECK : ~ leq (priv A e) l) :
         (forall a, secure_eqitF b1 b2 l vclo sim (observe t1) (observe (k2 a) )) ->
         secure_eqitF b1 b2 l vclo sim (observe t1) (VisF e k2)
+    (*| (halt : E A) k (Hempty : empty A) (r) : forall r', RR r' r -> eqit_secure (Vis halt k) (Ret r)
+
+     *)
   .
 
   Hint Constructors secure_eqitF : core.
@@ -94,8 +103,81 @@ Section SecureUntimed.
 
   Definition eqit_secure b1 b2 l := paco2 (secure_eqit_ b1 b2 l id) bot2.
 
+  (* want and eqitC_secure which could help prove some interesting stuff
+
+   *)
+
+
+  (*
+    Note that this is not reflexive (think it is symmetric and transitive) 
+    Suppose SecureFlip : E bool has privilege 1 and trigger SecureFlip is 
+    observed at privilege 0. We end to prove eqit_secure false false 0 of it 
+    requires us to show forall a b, eqit_secure false false 0 (Ret a) (Ret b)
+    this is false, suppose a = true and b = false and the relation is equality
+
+   *)
+
 
 End SecureUntimed.
+
+Definition NatPreorder : Preorder :=
+  {|
+  L := nat;
+  leq := fun n m => n <= m
+  |}.
+
+Section SecureUntimedUnReflexive.
+  
+  Variant NonDet : Type -> Type :=
+    | SecureFlip : NonDet bool
+    | PublicOut : NonDet unit
+    | Halt : NonDet void
+
+. 
+
+  Definition priv_counter : forall A, NonDet A -> nat :=
+    fun _ e =>
+      match e with
+      | SecureFlip => 1
+      | PublicOut => 0 
+      | Halt => 10
+      end.
+  
+
+  Variant Exc : Type -> Type :=
+    Throw : Exc void.
+
+  Definition refl_counter : itree NonDet bool := trigger SecureFlip.
+
+  Lemma refl_counter_counter : ~ eqit_secure NatPreorder priv_counter eq true true 0 refl_counter refl_counter.
+    Proof.
+      intro Hcontra. punfold Hcontra; try eapply secure_eqit_mono; eauto.
+      red in Hcontra. cbn in *. inv Hcontra; ITrace.inj_existT; subst.
+      - cbv in SECCHECK. inv SECCHECK.
+      - specialize (H0 true false). pclearbot. pinversion H0; try eapply secure_eqit_mono; eauto.
+        discriminate.
+      - rewrite H3 in H0. clear H3. specialize (H0 true). cbn in *.
+        inv H0; ITrace.inj_existT; subst. specialize (H2 false). rewrite H in H2.
+        inv H2. discriminate.
+      -  rewrite H in H0. injection H0; intros; ITrace.inj_existT; subst; ITrace.inj_existT; subst.
+         specialize (H1 true). cbn in *. inv H1; ITrace.inj_existT; subst; ITrace.inj_existT; subst.
+         rewrite H6 in H3. specialize (H3 false). cbn in *. inv H3; discriminate.
+    Qed.
+
+
+    Lemma halt_eq_all : forall R (t : itree NonDet R) k , eqit_secure NatPreorder priv_counter eq true true 0 (Vis Halt k) t.
+    Proof.
+      intros. pfold. red. cbn. constructor; auto; try intros; try contradiction.
+      intro Hc; inv Hc.
+    Qed.
+    (*transitivity problems in presence of E void *)
+    Definition refl_counter2 : itree NonDet unit := ITree.bind refl_counter (fun b : bool => if b then Ret tt else trigger PublicOut).
+
+    Lemma refl_counter2_counter : ~ eqit_secure NatPreorder priv_counter eq true true 0 refl_counter2 refl_counter2.
+      Proof.
+        Admitted.
+
+End SecureUntimedUnReflexive.
 
 Section SecureTimed.
 
